CertiGC/GC_Source/boxing.h
@@ -6,3 +6,4 @@ extern intnat int_or_ptr_to_int (value x); /* precondition: is int */
 extern void * int_or_ptr_to_ptr (value x); /* precond: is aligned ptr */
 extern value int_to_int_or_ptr(intnat x); /* precondition: is odd */
 extern value ptr_to_int_or_ptr(void *x); /* precondition: is aligned */
+extern int ptr_in_range(value* start, value * limit,  value * v);
