CertiGC/verif_gc.v
@@ -7,11 +7,6 @@ From CertiGraph.CertiGC Require Import
 
 Local Open Scope logic.
 
-Definition GC_imported_specs:funspecs := 
-  MallocASI ++
-  [spec_boxing.test_int_or_ptr_spec; spec_boxing.int_or_ptr_to_ptr_spec;
-   spec_boxing.ptr_to_int_or_ptr_spec].
-
 (*    spec_malloc.MallocASI ++ 
   [spec_boxing.test_int_or_ptr_spec; 
    (*spec_boxing.int_or_ptr_to_int_spec; *)
@@ -22,21 +17,154 @@ Definition GC_imported_specs:funspecs :=
 
 Definition GC_E : funspecs := nil.
 
-Require Import String.
+Definition GC_GP : globals -> mpred := all_string_constants Ers.
+
+Lemma init_data_tarray_tschar:
+  forall {cs : compspecs} sh (gv : globals) (b : block) (xs : list int) (i : ptrofs),
+  Ptrofs.unsigned i + Zlength xs < Ptrofs.modulus ->
+  init_data_list2pred gv (map Init_int8 xs) sh (Vptr b i)
+  |-- data_at sh (tarray tschar (Zlength xs)) (map Vint xs) (Vptr b i).
+Admitted.
+
+
+Definition ok_initbyte (b: init_data) : bool :=
+ match b with
+ | Init_int8 i => andb (negb (Z.eqb (Int.intval i) 0)) (andb (Z.leb (-128) (Int.intval i)) (Z.ltb (Int.intval i) 128))
+ | _ => false 
+ end.
+
+#[export] Instance Inhabitant_init_data: Inhabitant init_data := Init_int8 Int.zero.
+
+Lemma globvar2pred_cstring:
+ forall {cs: compspecs} gv i v,
+  headptr (gv i) ->
+  0 < Zlength (gvar_init v) < Ptrofs.modulus ->
+  Znth (Zlength (gvar_init v)-1) (gvar_init v) = Init_int8 Int.zero ->
+  gvar_volatile v = false ->
+  forallb ok_initbyte (sublist 0 (Zlength (gvar_init v)-1) (gvar_init v)) = true ->
+  gvar_info v = tarray tschar (Zlength (gvar_init v)) ->
+  (globvar2pred gv (i, v) |--
+  cstring (readonly2share (gvar_readonly v)) (map init_data2byte (sublist 0 (Zlength (gvar_init v)-1) (gvar_init v))) (gv i)).
+Proof.
+intros cs gv i v HEAD BOUND ZERO; intros.
+destruct HEAD as [b ?].
+destruct v;
+unfold globvar2pred; simpl in *.
+rewrite H; clear gvar_volatile H.
+rename gvar_init into bl0.
+set (bl := sublist 0 (Zlength bl0 - 1) bl0) in *.
+assert (exists al, map Init_int8 al = bl
+         /\ ~In Byte.zero (map (Basics.compose Byte.repr Int.intval) al)). {
+  clear - H0. clearbody bl.
+  induction bl. exists nil; auto.
+  simpl in H0.
+  destruct a; try discriminate H0.
+  rewrite andb_true_iff in H0. destruct H0.
+  destruct (IHbl H0) as [j [H3 H4]].
+  exists (i::j); simpl.
+  split.
+  f_equal. auto.
+  contradict H4. destruct H4; auto.
+  simpl in H.
+  exfalso; clear - H1 H.
+  rewrite !andb_true_iff in H; destruct H as [? [? ?]].
+  forget (Int.intval i) as j. clear i.
+  apply negb_true_iff, Z.eqb_neq in H. 
+  apply Z.leb_le in H0. apply Z.ltb_lt in H2.
+  assert (Byte.signed (Byte.repr j) = Byte.signed (Byte.zero)) by congruence.
+  rewrite Byte.signed_repr in H3 by rep_lia. contradiction.
+}
+rewrite H2.
+destruct H as [al [H3 H3']].
+subst bl.
+replace bl0 with (map Init_int8 (al ++ [Int.zero])). 
+ 2:{ rewrite map_app. rewrite H3.
+      simpl map. rewrite <- ZERO. list_solve.
+}
+eapply derives_trans.
+apply init_data_tarray_tschar.
+list_solve.
+unfold cstring.
+apply andp_right.
+apply prop_right.
+replace (map _ _) with (map (Byte.repr oo Int.intval) al); auto.
+autorewrite with sublist. rewrite sublist_map.
+rewrite sublist_app1 by rep_lia.
+rewrite sublist_same by lia.
+clear.
+induction al; simpl; auto. f_equal; auto.
+rewrite !Zlength_map.
+assert (map Vbyte (map init_data2byte (map Init_int8 al)) = map Vint al). {
+  rewrite <- H3 in H0.
+  clear - H0.
+  induction al; simpl in *; auto.
+  rewrite !andb_true_iff in H0.
+  destruct H0 as [[? [? ?]] ?].
+  f_equal; auto.
+  apply Z.leb_le in H0. apply Z.ltb_lt in H1.
+  unfold Vbyte. f_equal.
+  rewrite Byte.signed_repr by rep_lia.
+  change (Int.intval a) with (Int.unsigned a).
+  rewrite Int.repr_unsigned. auto.
+}
+autorewrite with sublist.
+apply derives_refl'.
+f_equal.
+rewrite sublist_map.
+autorewrite with sublist.
+rewrite !map_app.
+f_equal.
+auto.
+Qed.
+
+
+Lemma match_globals: 
+  forall gv : globals,
+  globals_ok gv -> 
+  InitGPred (Vardefs (QPprog gc_stack.prog) ) gv |-- all_string_constants Ers gv.
+Proof.
+intros.
+clear.
+unfold all_string_constants.
+repeat match goal with |- context [gv ?i] => progress (unfold i) end.
+set (j := Vardefs _); hnf in j; simpl in j; subst j.
+cbv [InitGPred fold_right map Maps.PTree.prev Maps.PTree.prev_append
+     globs2pred].
+Intros.
+rewrite !sepcon_assoc.
+apply sepcon_derives.
+apply derives_refl.
+
+repeat
+match goal with |- context [globvar2pred ?gv (?i, ?v)] =>
+  sep_apply (globvar2pred_cstring gv i v); [compute; split; reflexivity | ]
+end.
+clear.
+simpl.
+cancel.
+Qed.
+
+
+Ltac SF_vacuous ::= 
+ match goal with |- SF _ _ _ (vacuous_funspec _) => idtac end;
+ match goal with H: @eq compspecs _ _ |- _ => rewrite <- H end;
+red; red; repeat simple apply conj;
+[ reflexivity (* id_in_list ... *)
+| repeat apply Forall_cons; (* Forall complete_type fn_vars *)
+  try apply Forall_nil; reflexivity
+| repeat constructor; simpl; rep_lia (* var_sizes_ok *)
+| reflexivity (* fn_callconv ... *)
+| split3; [reflexivity | reflexivity | intros; apply semax_vacuous] (* semax_body *)
+| eexists; split; compute; reflexivity (* genv_find_func *)
+].
 
 Definition GCVSU: @VSU NullExtension.Espec
          GC_E GC_imported_specs ltac:(QPprog gc_stack.prog) 
-         spec_gc.GC_ASI (all_string_constants Ews).
+         spec_gc.GC_ASI GC_GP.
   Proof.
     mkVSU prog GC_Internal.
-intros.
-unfold Maps.PTree.prev in *; simpl in H.
-admit. (* need to take provide vacuous funspecs for,
-    garbage_collect_all certicoq_modify export_heap print_heapsize
-   reset_heap free_heap *)
     - solve_SF_internal body_is_ptr.
-    - admit.  (* Is_from *)
-    - admit. (* abort *)
+    - admit. (* abort_with *)
     - solve_SF_internal body_forward.
     - solve_SF_internal body_forward_roots.
     - admit. (* forward_remset *)
@@ -47,73 +175,6 @@ admit. (* need to take provide vacuous funspecs for,
     - solve_SF_internal body_make_tinfo.
     - solve_SF_internal body_resume. 
     - solve_SF_internal body_garbage_collect.
-    - admit. (* match up the string constants *)
+    - apply match_globals.
 all: fail.
 Admitted.
-(*
-intros. unfold Vardefs; simpl.
-unfold all_string_constants; simpl.
-unfold InitGPred; simpl.
-Intros.
-
-
-Search cstring.
-repeat
-match goal with |- context [globvar2pred ?gv (?i, ?v)] =>
-  let i' := eval hnf in i in
-  let v' := eval hnf in v in
-  let x := constr:(init_data_list2pred gv (gvar_init v') (readonly2share (gvar_readonly v')) (gv i')) in
-  let x' := eval cbv [gvar_init gvar_readonly readonly2share 
-                      init_data_list2pred init_data2pred init_data_size] in x in
-  change (globvar2pred gv (i,v)) with x'
-end.
-Print Ltac do_string2bytes.
-
-repeat change (Int.zero_ext 8 ?x) with x.
-simpl Int.zero_ext.
-simpl init_data_list2pred.
-
-   (init_data_list2pred gv (gvar_init v') (readonly2share (gvar_readonly v')) (gv i'));
-  
-end.
-unfold gvar_init, gvar_readonly, readonly2share.
-
-cbv [globvar2pred].
-repeat change (gvar_volatile _) with false.
-cbv match.
-
-simpl gvar_init.
-match goal with |- context [globvar2pred ?gv (?i, ?v)] =>
-
-change (globvar2pred _ (_, v___stderrp)) with emp.
-rewrite !sepcon_assoc.
-apply sepcon_derives. auto.
-apply sepcon_derives.
-{
-
-
-match goal with |- context [globvar2pred ?gv (?i, ?v)] =>
-  let i' := eval hnf in i in
-  let v' := eval hnf in v in 
-  change (globvar2pred gv (i,v)) with (globvar2pred gv (i',v'))
- end.
-
-unfold globvar2pred; simpl.
-
-
-rewrite !sepcon_assoc.
-repeat apply sepcon_derives.
-admit.  (* stderrp *)
-apply derives
-f_equal.
-unfold globvar2pred.
-simpl gvar_volatile; cbv match.
-simpl gvar_init.
-simpl fst.
-
-entailer!!.
-cancel.
-
- subst p; simpl. apply derives_refl. solve_SF_internal 
-    - 
-*)
