CertiGC/verif_boxing.v
@@ -4,6 +4,8 @@ Local Open Scope logic.
 
 Axiom body_test_int_or_ptr: semax_body Vprog Gprog f_test_int_or_ptr test_int_or_ptr_spec.
 
+Axiom body_ptr_in_range: semax_body Vprog Gprog f_ptr_in_range ptr_in_range_spec.
+
 Lemma body_int_to_int_or_ptr:
   semax_body Vprog Gprog f_int_to_int_or_ptr int_to_int_or_ptr_spec.
 Proof.
@@ -46,4 +48,5 @@ Definition BoxingVSU: @VSU NullExtension.Espec
     - solve_SF_internal body_int_or_ptr_to_ptr.
     - solve_SF_internal body_int_to_int_or_ptr.
     - solve_SF_internal body_ptr_to_int_or_ptr.
+    - solve_SF_internal body_ptr_in_range.
 Qed.
